vyperTestScript.sml
@@ -11,10 +11,10 @@ Definition test_if_control_flow_ast_def:
     AnnAssign "a" (UintT (n2w (256 DIV 8))) (Literal (IntL 1));
     If (Compare (Name "a") Eq (Literal (IntL 1)))
     [
-      Assign "a" (Literal (IntL 2))
+      Assign (BaseTarget (NameTarget "a")) (Literal (IntL 2))
     ]
     [
-      Assign "a" (Literal (IntL 3))
+      Assign (BaseTarget (NameTarget "a")) (Literal (IntL 3))
     ];
     Return (SOME (BinOp (Name "a") Add (Literal (IntL 42))))
   ] (UintT (n2w (256 DIV 8)))
@@ -30,7 +30,8 @@ Proof
   rw[function_body_def, test_if_control_flow_ast_def]
   \\ simp[execute_stmts_def, new_variable_def,
           initial_function_context_def,
-          evaluate_exps_def, assign_target_def,
+          evaluate_exps_def, assign_target_def, set_variable_def,
+          evaluate_target_def, evaluate_base_target_def,
           evaluate_cmp_def, evaluate_literal_def,
           evaluate_binop_def, lookup_scopes_def,
           find_containing_scope_def,
@@ -45,7 +46,7 @@ Definition test_for_control_flow_ast_def:
        (ArrayLit [Literal (IntL 1); Literal (IntL 2); Literal (IntL 3)]);
      AnnAssign "counter" (UintT (n2w (256 DIV 8))) (Literal (IntL 0));
      For "i" (UintT (n2w (256 DIV 8))) (Name "a")
-     [ OpAssign "counter" Add (Name "i") ];
+     [ AugAssign "counter" Add (Name "i") ];
      Return (SOME (Name "counter"))
   ] (UintT (n2w (256 DIV 8)))
 End
@@ -60,11 +61,27 @@ Proof
   rw[function_body_def, test_for_control_flow_ast_def]
   \\ simp[execute_stmts_def,
        initial_function_context_def, new_variable_def,
+       set_variable_def, evaluate_base_target_def, evaluate_target_def,
        evaluate_exps_def, assign_target_def,
        evaluate_cmp_def, evaluate_literal_def,
        evaluate_binop_def, push_scope_def, lookup_scopes_def,
        find_containing_scope_def, pop_scope_def,
        raise_def, FLOOKUP_UPDATE]
 QED
+
+Definition test_array_assign_ast_def:
+  test_array_assign_ast =
+  FunctionDef "foo" [External] []
+  [
+    AnnAssign "bar" (DynArrayT (UintT (n2w (256 DIV 8))) 10)
+      (ArrayLit [Literal (IntL 1); Literal (IntL 2)]);
+    Assign (BaseTarget (SubscriptTarget (NameTarget "bar") (Literal (IntL 0))))
+      (Literal (IntL 3));
+    Return (SOME (BinOp (BinOp (Subscript (Name "bar") (Literal (IntL 0))) Add
+                               (Subscript (Name "bar") (Literal (IntL 1)))) Add
+                        (Literal (IntL 42))))
+
+  ]
+End
 
 val () = export_theory();
